semantics/replScript.sml
@@ -16,7 +16,7 @@ repl_state = <| (* Elaborator state *)
 
 val init_repl_state_def = Define`
   init_repl_state = <| type_bindings := init_type_bindings; ctors := [];
-                       tdecs := ({},{},{}); tenvM := []; tenvC := init_tenvC; tenv := init_tenv;
+                       tdecs := init_decls; tenvM := []; tenvC := init_tenvC; tenv := init_tenv;
                        envM := []; envC := init_envC; store := ([],{},{}); envE := init_env |>`
 
 val _ = Hol_datatype `
